src/Config.fst
@@ -1,0 +1,9 @@
+module Config
+
+open Prelude
+
+let metadata_max = 131072ul
+
+let alg_null = U32.v metadata_max + 1
+
+let alg_null_sizet = US.of_u32 131073ul
