src/Config.fsti
@@ -1,0 +1,20 @@
+module Config
+
+module U64 = FStar.UInt64
+module U32 = FStar.UInt32
+module US = FStar.SizeT
+
+open FStar.Mul
+
+// LATER: code could be improved so that this value is not hardcoded anymore
+inline_for_extraction
+let page_size: U32.t = 4096ul
+
+// LATER: this should likely be a sizet
+inline_for_extraction
+val metadata_max: v:U32.t{FStar.UInt.size (U32.v v * U32.v page_size) 32}
+
+noextract inline_for_extraction
+val alg_null: v:nat{v = U32.v metadata_max + 1}
+noextract inline_for_extraction
+val alg_null_sizet: v:US.t{US.v v = U32.v metadata_max + 1}
