src/Main.fst
@@ -22,6 +22,8 @@ open SizeClass
 open SlabsCommon
 open SteelVRefineDep
 open SteelStarSeqUtils
+
+open Config
 open Utils2
 
 
